Use stdpp; compiles

lib/Algebra.v
@@ -1,13 +1,5 @@
-Require Import Coqlib sflib.
-
-(*** From stdpp ***)
-Class Equiv (A: Type) := equiv: A -> A -> Prop.
-Global Instance equiv_rewrite_relation `{Equiv A} :
-  RewriteRelation (@equiv A _) | 150 := {}.
-Notation "≡" := equiv (at level 70).
-Infix "≡" := equiv (at level 70, no associativity).
-Infix "≡@{ A }" := (@equiv A _)
-  (at level 70, only parsing, no associativity).
+Require Import Coqlib sflib String.
+From stdpp Require Export base tactics.
 
 Class OPlus (T: Type) := oplus: T -> T -> T.
 Notation "(⊕)" := oplus (at level 50).
@@ -17,28 +9,33 @@ Class Bar (T: Type) := bar: T -> T.
 Notation "|-|" := bar (at level 50).
 Notation "| a |" := (bar a) (at level 50).
 
-Class Ref (T: Type) := ref : T -> T -> Prop.
+(* Notation "'ref'" := sqsubseteq (at level 60, only parsing). *)
+Notation "'Ref'" := SqSubsetEq (at level 60, only parsing).
+Definition ref_both `{Ref T}: T -> T -> Prop := λ a b, a ⊑ b /\ b ⊑ a.
 
-Definition ref_both `{Ref T}: T -> T -> Prop := fun a b => ref a b /\ ref b a.
+(* Notation "⊒⊑" := ref_both (at level 70). *)
+(* Notation "a ⊒⊑ b" := (ref_both a b) (at level 70). *)
+Infix "⊒⊑" := ref_both (at level 70) : stdpp_scope.
+Notation "(⊒⊑)" := ref_both (only parsing) : stdpp_scope.
+Notation "( x ⊒⊑.)" := (ref_both x) (only parsing) : stdpp_scope.
+Notation "(.⊒⊑ y )" := (λ x, ref_both x y) (only parsing) : stdpp_scope.
 
-Notation "⊑" := ref (at level 70).
-Notation "a ⊑ b" := (ref a b) (at level 70).
-Notation "⊒⊑" := ref_both (at level 60).
-Notation "a ⊒⊑ b" := (ref_both a b) (at level 60).
+Infix "⊒⊑@{ A }" := (@ref_both A _) (at level 70, only parsing) : stdpp_scope.
+Notation "(⊒⊑@{ A } )" := (@ref_both A _) (only parsing) : stdpp_scope.
 
-Global Program Instance ref_both_ref `{Ref T}: subrelation ((⊒⊑)) ((⊑)).
+Global Program Instance ref_both_ref `{Ref T}: subrelation ((⊒⊑)) ((⊑@{T})).
 Next Obligation.
-  rr in H0. des; eauto.
+  i. rr in H0. des; eauto.
 Qed.
 
-Global Program Instance ref_both_ref2 `{Ref T}: subrelation ((⊒⊑)) (flip (⊑)).
+Global Program Instance ref_both_ref2 `{Ref T}: subrelation ((⊒⊑)) (flip (⊑@{T})).
 Next Obligation.
-  rr in H0. des; eauto.
+  i. rr in H0. des; eauto.
 Qed.
 
 Global Program Instance equiv_ref_both `{Equiv T, Ref T, !Symmetric (≡), !subrelation (≡) (⊑)}: subrelation (≡) (⊒⊑).
 Next Obligation.
-  rr. esplits; et.
+  i. rr. esplits; et.
 Qed.
 
 Class Eps (T: Type) := eps : T.
@@ -47,20 +44,20 @@ Notation "'ε'" := eps.
 Class EquivFacts `{Equiv T} := equiv_facts:> Equivalence ((≡)).
 
 Class RefFacts `{Equiv T, Ref T, OPlus T} := {
-    ref_Preorder:> PreOrder ((⊑));
+    ref_Preorder:> PreOrder ((⊑@{T}));
     ref_oplus:> Proper ((⊑) ==> (⊑) ==> (⊑)) ((⊕));
     ref_equiv:> subrelation ((≡)) ((⊑));
 }.
 
 Global Program Instance ref_Proper `{Equiv T, Ref T, OPlus T, !RefFacts, !EquivFacts}: Proper ((≡) ==> (≡) ==> impl) ((⊑)).
 Next Obligation.
-  ii. etrans; et.
-  { eapply ref_equiv; et. sym; et. }
+  ii. etrans.
+  { eapply ref_equiv. sym; et. }
   etrans; et.
   { eapply ref_equiv; et. }
 Qed.
 
-Global Program Instance ref_both_Equivalence `{Equiv T, Ref T, OPlus T} `{!EquivFacts} `{!RefFacts}: Equivalence ((⊒⊑)).
+Global Program Instance ref_both_Equivalence `{Equiv T, Ref T, OPlus T} `{!EquivFacts} `{!RefFacts}: Equivalence ((⊒⊑@{T})).
 Next Obligation.
   ii. rr. esplits; try refl.
 Qed.
@@ -96,8 +93,8 @@ Class BarFactsWeak `{Equiv T, Bar T, OPlus T, Ref T} := {
 }.
 
 Global Program Instance BarFactsWeaken `{Equiv T, Bar T, OPlus T, Ref T, !EquivFacts, !BarFacts, !RefFacts}: BarFactsWeak.
-Next Obligation. rewrite bar_idemp. refl. Qed.
-Next Obligation. rewrite bar_oplus. refl. Qed.
+Next Obligation. i. rewrite bar_idemp. refl. Qed.
+Next Obligation. i. rewrite bar_oplus. refl. Qed.
 
 (* Class OPlusFacts `{Equiv T, OPlus T, Ref T} `{EQVF: EquivFacts T} `{@RefFacts _ _ EQVF _ _} := { *)
 Class OPlusFacts `{Equiv T, OPlus T} := {
@@ -113,10 +110,10 @@ Class OPlusFactsWeak `{Equiv T, OPlus T, Ref T} := {
 }.
 
 Global Program Instance OPlusFactsWeaken `{Equiv T, OPlus T, Ref T, !EquivFacts, !OPlusFacts, !RefFacts}: OPlusFactsWeak.
-Next Obligation. rewrite oplus_comm. refl. Qed.
-Next Obligation. rewrite oplus_assoc. refl. Qed.
+Next Obligation. i. rewrite oplus_comm. refl. Qed.
+Next Obligation. i. rewrite oplus_assoc. refl. Qed.
 
-Lemma oplus_assoc_weak2 `{Equiv T, OPlus T, Ref T, !OPlusFactsWeak, !PreOrder ((⊑))}: forall a b c, (a ⊕ b) ⊕ c ⊑ a ⊕ (b ⊕ c).
+Lemma oplus_assoc_weak2 `{Equiv T, OPlus T, Ref T, !OPlusFactsWeak, !PreOrder ((⊑@{T}))}: forall a b c, (a ⊕ b) ⊕ c ⊑ a ⊕ (b ⊕ c).
 Proof.
   ii. rewrite oplus_comm_weak. rewrite oplus_assoc_weak. rewrite oplus_comm_weak. rewrite oplus_assoc_weak.
   rewrite oplus_comm_weak. refl.
@@ -196,10 +193,10 @@ Global Instance Bar_pointed `{Bar T}: Bar (pointed T) :=
 
 Ltac upt :=
   repeat match goal with
-    | [H: context[@Algebra.equiv _ (@Equiv_pointed _ _)] |- _] => unfold Algebra.equiv, Equiv_pointed in H
-    | [ |- context[@Algebra.equiv _ (@Equiv_pointed _ _)]] => unfold Algebra.equiv, Equiv_pointed
-    | [H: context[@Algebra.ref _ (@Ref_pointed _ _)] |- _] => unfold Algebra.ref, Ref_pointed in H
-    | [ |- context[@Algebra.ref _ (@Ref_pointed _ _)]] => unfold Algebra.ref, Ref_pointed
+    | [H: context[@equiv _ (@Equiv_pointed _ _)] |- _] => unfold equiv, Equiv_pointed in H
+    | [ |- context[@equiv _ (@Equiv_pointed _ _)]] => unfold equiv, Equiv_pointed
+    | [H: context[@sqsubseteq _ (@Ref_pointed _ _)] |- _] => unfold sqsubseteq, Ref_pointed in H
+    | [ |- context[@sqsubseteq _ (@Ref_pointed _ _)]] => unfold sqsubseteq, Ref_pointed
     | [H: context[@Algebra.bar _ (@Bar_pointed _ _)] |- _] => unfold Algebra.bar, Bar_pointed in H
     | [ |- context[@Algebra.bar _ (@Bar_pointed _ _)]] => unfold Algebra.bar, Bar_pointed
     | [H: context[@Algebra.eps _ (@Eps_pointed _ _)] |- _] => unfold Algebra.eps, Eps_pointed in H
@@ -304,8 +301,144 @@ Class RefBFacts `{Equiv T, Ref T, RefB T} := {
 Global Program Instance refB_Proper
   `{Equiv T, Ref T, RefB T, OPlus T, !RefBFacts, !EquivFacts}: Proper ((≡) ==> (≡) ==> impl) ((⊑B)).
 Next Obligation.
-  ii. etrans; et.
-  { eapply refb_equiv; et. sym; et. }
+  ii. etrans.
+  { eapply refb_equiv. sym; et. }
   etrans; et.
   { eapply refb_equiv; et. }
 Qed.
+
+
+
+Module MRAS.
+
+  Class t: Type := {
+    car:> Type;
+    equiv:> Equiv car;
+    oplus:> OPlus car;
+    ref:> Ref car;
+    bar:> Bar car;
+    eps:> Eps car;
+    equiv_facts:> EquivFacts (T:=car);
+    ref_facts:> RefFacts (T:=car);
+    oplus_facts:> OPlusFacts (T:=car);
+    bar_facts:> BarFacts (T:=car);
+    eps_facts:> EpsFacts (T:=car);
+    affinity: forall a, a ⊑ ε;
+    bar_intro: forall a, a ⊑ a ⊕ |a|;
+  }.
+
+End MRAS.
+
+Global Instance equiv_relaxed `{M: MRA.t}: Equiv _ | 100
+  := fun a b => a ⊒⊑ b /\ |a| ⊒⊑ |b|.
+
+Global Program Instance MRA_to_MRAS (M: MRA.t): MRAS.t := {
+  car := MRA.car;
+  equiv := equiv_relaxed;
+}.
+Next Obligation.
+  econs.
+  - ii; ss.
+  - ii; ss. rr in H. des. rr. esplits; sym; et.
+  - ii; ss. rr in H. rr in H0. des. rr. esplits; etrans; et.
+Qed.
+Next Obligation.
+  econs; try typeclasses eauto.
+  ii. rr in H. des; ss. eapply H.
+Qed.
+Next Obligation.
+  econs; try typeclasses eauto.
+  - ii. rr. esplits; et.
+    + r. esplits; eapply oplus_comm_weak.
+    + rewrite ! bar_oplus_weak. r. esplits; eapply oplus_comm_weak.
+  - ii. rr. esplits; et.
+    + r. esplits; try eapply oplus_assoc_weak; try eapply oplus_assoc_weak2.
+    + rewrite ! bar_oplus_weak. r.
+      esplits; try eapply oplus_assoc_weak; try eapply oplus_assoc_weak2.
+  - ii. rr in H. rr in H0. des. rr. esplits; et.
+    + rewrite H. rewrite H0. refl.
+    + rewrite ! bar_oplus_weak.
+      rewrite H1. rewrite H2. refl.
+Qed.
+Next Obligation.
+  econs; try typeclasses eauto.
+  - ii. rr. esplits; et.
+    + rewrite bar_idemp_weak. refl.
+    + rewrite bar_idemp_weak. refl.
+  - ii. rr. esplits.
+    + rewrite bar_oplus_weak. refl.
+    + rewrite bar_idemp_weak. rewrite ! bar_oplus_weak.
+      rewrite ! bar_idemp_weak.
+      refl.
+  - ii. rr in H. des. rr. esplits; et.
+    + rewrite ! bar_idemp_weak. ss.
+Qed.
+Next Obligation.
+  econs; try typeclasses eauto.
+  - ii. rr. esplits; et.
+    + rewrite eps_r. refl.
+    + rewrite bar_oplus_weak. rewrite eps_bar. rewrite eps_r. refl.
+  - ii. rr. esplits; et.
+    + rewrite eps_l. refl.
+    + rewrite bar_oplus_weak. rewrite eps_bar. rewrite eps_l. refl.
+  - rr. esplits; try rewrite ! eps_bar; refl.
+Qed.
+Next Obligation.
+  i. eapply MRA.affinity.
+Qed.
+Next Obligation.
+  i. eapply MRA.bar_intro.
+Qed.
+
+Global Program Instance hat_Proper `{MRA.t}: Proper ((≡) ==> equiv_relaxed) (fun x => x).
+Next Obligation.
+  ii. rr. esplits.
+  - rewrite H0. refl.
+  - rewrite H0. refl.
+Qed.
+
+Definition included `{OPlus T, Equiv T}: T -> T -> Prop :=
+  fun a b => exists ctx, (a ⊕ ctx) ≡ b.
+Notation "(≼)" := (included) (at level 50).
+Notation "x ≼ y" := (included x y) (at level 50).
+
+Section INCLUDEDFACTS.
+
+  Context `{M: MRAS.t}.
+
+  Global Program Instance included_sub :
+    subrelation ((≡)) ((≼)).
+  Next Obligation.
+    ii; ss. r. exists ε. rewrite eps_r. ss.
+  Qed.
+
+  Global Program Instance included_Proper: Proper ((≡) ==> (≡) ==> impl) ((≼)).
+  Next Obligation.
+    ii; ss. r in H1. r. des. setoid_subst. et.
+  Qed.
+
+  Global Program Instance included_PreOrder: PreOrder ((≼)).
+  Next Obligation.
+    ii. rr. esplits; et. rewrite eps_r. refl.
+  Qed.
+  Next Obligation.
+    unfold included. ii. des. esplits; et. setoid_subst. rewrite oplus_assoc. f_equal.
+  Qed.
+
+  Global Program Instance oplus_included: Proper ((≼) ==> (≼) ==> (≼)) ((⊕)).
+  Next Obligation.
+    unfold included.
+    ii. des. setoid_subst. esplits; et. rewrite <- ! oplus_assoc. f_equiv.
+    instantiate (1:=ctx0 ⊕ ctx).
+    rewrite ! oplus_assoc. f_equiv.
+    rewrite oplus_comm. f_equiv.
+  Qed.
+
+  Lemma unit_included: ∀ x, ε ≼ x.
+  Proof.
+    ii. r. esplits. rewrite eps_l. refl.
+  Qed.
+
+End INCLUDEDFACTS.
+
+
